ecAdd wip

examples/ecAdd/proofs/AlmostYUL.ec
@@ -1,40 +1,61 @@
-require import AllCore Int IntDiv.
+require import AllCore Int IntDiv Gcd_props.
 
 op R2_MOD_P : int.
 op R, N, N' : int.
 
 op getHighestHalfOfMultiplication (a b : int) : int = (a * b) %/ R.
+op as_bool (b : bool) = b.
 
 
 module AlmostYul = {
 
+  proc addmod(a : int, b : int, modulus : int) : int = {
+    var sum <- (a + b) %% R  %% modulus;
+    return sum;
+  }
+
+  proc submod(minuend : int, subtrahend : int, modulus : int) : int = {
+    var difference;
+    difference <@ addmod(minuend, (modulus - subtrahend) %% R, modulus);
+    return difference;
+  }
+
+  proc getHighestHalfOfMultiplication(a : int, b : int) : int = {
+   return getHighestHalfOfMultiplication a b; 
+  }
 
   proc overflowingAdd(augend : int, addend : int, R : int) : int * bool = {
     var sum <- (augend + addend) %% R;
     return (sum, sum < augend);
   }
 
+
+   proc isInfinity(x : int, y : int) : bool = {
+       return x = 0 /\ y = 0;
+   }
+
+  proc isOnFieldOrder(coordinate : int) : bool = {
+      return coordinate < N;
+  }
+
+
+
+
   proc _REDC(Tlo : int, Thi : int, R : int, N : int, N' : int) = {
     var m, hi, lo, s, tmp, overflowed;
-
     m <- (Tlo * N') %% R;
-     
     hi <- (Thi + ((m * N) %/ R)) %% R;
     tmp <- (m * N) %% R;
-     
     (lo, overflowed) <@ overflowingAdd(Tlo, tmp, R);
     if (overflowed) {
       hi <- (hi + 1) %% R;
     }
-
     s <- hi;
-
     if (N <= hi){
       s <- (hi - N) %% R;
     }
     return s;
   } 
-
 
 
   proc outOfMontgomeryForm(m : int) : int = {
@@ -45,11 +66,9 @@ module AlmostYul = {
 
   proc intoMontgomeryForm(a : int) : int = {
       var ret, hi, lo;
-
       hi <- getHighestHalfOfMultiplication a R2_MOD_P;
       lo <- (a * R2_MOD_P) %% R;
-      ret <@ _REDC(lo, hi, R, N, N');
-    
+      ret <@ _REDC(lo, hi, R, N, N');    
       return ret;
   }
 
@@ -76,4 +95,323 @@ module AlmostYul = {
     return ret;
   }
 
+
+
+  proc simplify_ts_pos(t2:int,t3: int,u:int) = {
+      while (even t3){
+        if (even t2){
+          (t2,t3) <- (t2 %/2, t3 %/2);
+        }else{
+          (t2,t3) <- ((t2+u) %% R %/2, t3 %/2);
+        }
+      }
+      return (t2,t3);
+  }
+
+
+  proc binaryExtendedEuclideanAlgorithm(u : int, v : int, r : int) = {
+    var u2,u3,v2,v3,t2,t3;
+
+    (u2,u3) <- (0, u);
+    (v2,v3) <- (r, v);
+    (t2,t3) <- (r, v);
+
+    (t2,t3) <@ simplify_ts_pos(t2, v, u);
+    (v2, v3) <- (t2, t3);
+
+    if (v3 < u3){
+      t3 <- (u3 - v3) %% R;
+    }else{
+      t3 <- (v3 - u3) %% R;
+    }
+    t2 <- v2;
+
+    while (t3 <> 0){
+      (t2,t3) <@ simplify_ts_pos(t2, t3, u);
+
+      if (v3 < u3){
+        (u2, u3) <- (t2, t3);
+      }else{
+        (v2, v3) <- (t2, t3);
+      }
+
+      t2 <- u2 + v2;
+      if (u <= t2){
+          t2 <- (t2 - u) %% R;
+      }else{
+          t2 <- (u2 + v2) %% R;
+      }
+
+      if (v3 < u3){
+        t3 <- (u3 - v3) %% R;
+      }else{
+        t3 <- (v3 - u3) %% R;
+      }
+
+     }
+    return (u-u2) %% R;
+  }
+
+
+  proc montgomeryModularInverse(a : int) : int = {
+    var invmod;
+    invmod <@ binaryExtendedEuclideanAlgorithm(N,a,R2_MOD_P);
+    return invmod;
+  } 
+
+ proc montgomeryDiv(dividend : int, divisor: int) : int = {
+   var quotient, inverse;
+   inverse  <@ montgomeryModularInverse(divisor);
+   quotient <@ montgomeryMul(dividend, inverse);
+   return quotient;
+ }
+
+
+ proc pointIsInCurve(x: int, y: int) : bool = {
+  var ySquared, xSquared, xQubed, xQubedPlusThree;
+  ySquared <@ montgomeryMul(y, y);
+  xSquared <@ montgomeryMul(x, x);
+  xQubed <@ montgomeryMul(xSquared, x);
+  xQubedPlusThree <@ montgomeryAdd(xQubed, (3 * R) %% N);
+  return (ySquared = xQubedPlusThree);    
+ }
+
+proc and(b1:bool, b2:bool) : bool = {
+   return b1 /\ b2;
+}
+
+
+proc or(b1:bool, b2:bool) : bool = {
+   return b1 \/ b2;
+}
+
+proc eq(b1:int, b2:int) : bool = {
+   return b1 = b2;
+}
+
+
+proc iszero(b) : bool = {
+   return !b;
+}
+
+proc burnGas() = {
+  while(true){}
+}
+
+proc _P() : int = {
+ return N;
+}    
+
+
+proc main(x1: int, y1: int, x2: int, y2: int) : int * int = { 
+        var ret, p1IsInfinity, p2IsInfinity, func17, func43, func47, func53, func55, func57, func61, func63, m_x2, m_y2, func79, func81, func109, func111, func119, func121, func123, func127, func129, m_x1, m_y1, func145, func147, func175, func177, func179, func183, func185, func193, func195, func197, func201, func203, func211, func213, func219, func221, func227, func249, func251, func253, func259, func261, func289, func291, func297, func299, func301, func307, func309, func313, func319, func325, func327, func333, x, y, func349, func351, x1_squared, slope, func368, func372, func378, func380, func382, func388, x3, func392, func398, func404, func406, y3, func410, func414, func420, func424, func469, func471, func473, func479, func481, func492, func498, func500, func506, func510, func516, func522, func524, func528, func532, func538, func542, ret_bool;
+        ret_bool <- false;
+
+        p1IsInfinity <@ isInfinity(x1,y1);
+        p2IsInfinity <@ isInfinity(x2,y2);
+        func17 <@ and(p1IsInfinity,p2IsInfinity);
+        if(as_bool func17){
+            ret <- (0,0);
+            ret_bool <- true;
+
+        }
+
+        if (!ret_bool){
+
+        func47 <@ iszero(p2IsInfinity);
+        func43 <@ and(p1IsInfinity,func47);
+        if(as_bool func43){
+            func57 <@ isOnFieldOrder(x2);
+            func55 <@ iszero(func57);
+            func63 <@ isOnFieldOrder(y2);
+            func61 <@ iszero(func63);
+            func53 <@ or(func55,func61);
+            if(as_bool func53){
+                burnGas();
+
+            }
+            m_x2 <@ intoMontgomeryForm(x2);
+            m_y2 <@ intoMontgomeryForm(y2);
+            func81 <@ pointIsInCurve(m_x2,m_y2);
+            func79 <@ iszero(func81);
+            if(as_bool func79){
+                burnGas();
+
+            }
+            ret <- (x2,y2);
+            ret_bool <- true;
+
+        }
+
+        if (!ret_bool) {
+
+        func111 <@ iszero(p1IsInfinity);
+        func109 <@ and(func111,p2IsInfinity);
+        if(as_bool func109){
+            func123 <@ isOnFieldOrder(x1);
+            func121 <@ iszero(func123);
+            func129 <@ isOnFieldOrder(y1);
+            func127 <@ iszero(func129);
+            func119 <@ or(func121,func127);
+            if(as_bool func119){
+                burnGas();
+
+            }
+            m_x1 <@ intoMontgomeryForm(x1);
+            m_y1 <@ intoMontgomeryForm(y1);
+            func147 <@ pointIsInCurve(m_x1,m_y1);
+            func145 <@ iszero(func147);
+            if(as_bool func145){
+                burnGas();
+
+            }
+            ret <- (x1,y1);
+            ret_bool <- true;
+
+        }
+
+        if (!ret_bool) {
+
+        func179 <@ isOnFieldOrder(x1);
+        func177 <@ iszero(func179);
+        func185 <@ isOnFieldOrder(y1);
+        func183 <@ iszero(func185);
+        func175 <@ or(func177,func183);
+        if(as_bool func175){
+            burnGas();
+
+        }
+        func197 <@ isOnFieldOrder(x2);
+        func195 <@ iszero(func197);
+        func203 <@ isOnFieldOrder(y2);
+        func201 <@ iszero(func203);
+        func193 <@ or(func195,func201);
+        if(as_bool func193){
+            burnGas();
+
+        }
+        func213 <@ eq(x1,x2);
+        func227 <@ _P();
+        func221 <@ submod(0,y1,func227);
+        func219 <@ eq(func221,y2);
+        func211 <@ and(func213,func219);
+        if(as_bool func211){
+            m_x1 <@ intoMontgomeryForm(x1);
+            m_y1 <@ intoMontgomeryForm(y1);
+            m_x2 <@ intoMontgomeryForm(x2);
+            m_y2 <@ intoMontgomeryForm(y2);
+            func253 <@ pointIsInCurve(m_x1,m_y1);
+            func251 <@ iszero(func253);
+            func261 <@ pointIsInCurve(m_x2,m_y2);
+            func259 <@ iszero(func261);
+            func249 <@ or(func251,func259);
+            if(as_bool func249){
+                burnGas();
+
+            }
+            ret <- (0,0);
+            ret_bool <- true;            
+        }
+
+        if (!ret_bool){
+
+        func291 <@ eq(x1,x2);
+        func301 <@ eq(y1,y2);
+        func299 <@ iszero(func301);
+        func319 <@ _P();
+        func313 <@ submod(0,y2,func319);
+        func309 <@ eq(y1,func313);
+        func307 <@ iszero(func309);
+        func297 <@ and(func299,func307);
+        func289 <@ and(func291,func297);
+        if(as_bool func289){
+            burnGas();
+
+        }
+        func327 <@ eq(x1,x2);
+        func333 <@ eq(y1,y2);
+        func325 <@ and(func327,func333);
+        if(as_bool func325){
+            x <@ intoMontgomeryForm(x1);
+            y <@ intoMontgomeryForm(y1);
+            func351 <@ pointIsInCurve(x,y);
+            func349 <@ iszero(func351);
+            if(as_bool func349){
+                burnGas();
+
+            }
+            x1_squared <@ montgomeryMul(x,x);
+            func378 <@ _P();
+            func372 <@ addmod(x1_squared,x1_squared,func378);
+            func380 <@ _P();
+            func368 <@ addmod(x1_squared,func372,func380);
+            func388 <@ _P();
+            func382 <@ addmod(y,y,func388);
+            slope <@ montgomeryDiv(func368,func382);
+            func392 <@ montgomeryMul(slope,slope);
+            func404 <@ _P();
+            func398 <@ addmod(x,x,func404);
+            func406 <@ _P();
+            x3 <@ submod(func392,func398,func406);
+            func420 <@ _P();
+            func414 <@ submod(x,x3,func420);
+            func410 <@ montgomeryMul(slope,func414);
+            func424 <@ _P();
+            y3 <@ submod(func410,y,func424);
+            x3 <@ outOfMontgomeryForm(x3);
+            y3 <@ outOfMontgomeryForm(y3);
+
+            ret <- (x3,y3);
+            ret_bool <- true;
+        }
+
+        if (!ret_bool) {
+
+        x1 <@ intoMontgomeryForm(x1);
+        y1 <@ intoMontgomeryForm(y1);
+        x2 <@ intoMontgomeryForm(x2);
+        y2 <@ intoMontgomeryForm(y2);
+        func473 <@ pointIsInCurve(x1,y1);
+        func471 <@ iszero(func473);
+        func481 <@ pointIsInCurve(x2,y2);
+        func479 <@ iszero(func481);
+        func469 <@ or(func471,func479);
+        if(as_bool func469){
+            burnGas();
+
+        }
+        func498 <@ _P();
+        func492 <@ submod(y2,y1,func498);
+        func506 <@ _P();
+        func500 <@ submod(x2,x1,func506);
+        slope <@ montgomeryDiv(func492,func500);
+        func510 <@ montgomeryMul(slope,slope);
+        func522 <@ _P();
+        func516 <@ addmod(x1,x2,func522);
+        func524 <@ _P();
+        x3 <@ submod(func510,func516,func524);
+        func538 <@ _P();
+        func532 <@ submod(x1,x3,func538);
+        func528 <@ montgomeryMul(slope,func532);
+        func542 <@ _P();
+        y3 <@ submod(func528,y1,func542);
+        x3 <@ outOfMontgomeryForm(x3);
+        y3 <@ outOfMontgomeryForm(y3);
+
+        ret <- (x3,y3);
+
+        }
+        }
+        }
+        }
+        }
+
+        return ret;
+    }
+
+
+
+
 }.
+
+
