examples/ecAdd/proofs/montgomery_arith.ec
@@ -13,6 +13,34 @@ axiom ax4 :  coprime P R.
 axiom R_pos : 0 < R. 
 axiom ax5 : 0 <= R2_MOD_P < P.
 axiom ax6 : R2_MOD_P = (R * R) %% P.
+axiom ax7 : 2 < P.
+axiom ax9 : odd P.
+axiom ax10 : odd R2_MOD_P.
+axiom P_prime : prime P.
+
+axiom ax11 (a b : int) : coprime P (a * b) => inv P (a * b) %% P  = inv P a * inv P b %% P.
+axiom ax12 a : coprime P a => inv P (a %% P) = inv P a.
+lemma ax13 a : coprime P a = coprime P (a %% P). rewrite /coprime. rewrite gcd4. rewrite - gcd_modl.
+rewrite gcd4. auto. qed.
+
+
+
+lemma addmod a_in b_in m_in :
+    phoare [ AlmostYul.addmod : arg = (a_in,b_in,m_in)  /\ 0 <= a_in < m_in /\ 0 <= 2 * m_in < R
+      /\  0 <= b_in <= m_in ==> res = (a_in + b_in) %% m_in ] = 1%r.
+proof. proc.
+wp. skip. progress. smt.
+qed.
+
+
+lemma submod a_in b_in m_in :
+    phoare [ AlmostYul.submod : arg = (a_in,b_in,m_in)  /\ 0 <= a_in < m_in /\ 0 <= 2 * m_in < R
+      /\  0 <= b_in <= m_in ==> res = (a_in - b_in) %% m_in ] = 1%r.
+proof. proc.
+call (addmod a_in ((m_in - b_in) %% R) m_in). skip. progress.
+smt. smt. smt.
+qed.
+
 
 op comb (l h : int) = h * R + l.
 
@@ -26,14 +54,18 @@ qed.
     
 
 lemma almost_yul_redc_full_correctness':
-  forall (Tlo Thi R_in N' N : int),
-    2 * N < R_in =>
+  forall (Tlo Thi  N' N : int),
+    2 * N < AlmostYUL.R =>
     0 < N =>
-    N' * N %% R_in = (-1) %% R_in =>
-    coprime N R_in =>
+    N' * N %% AlmostYUL.R = (-1) %% AlmostYUL.R =>
+    coprime N AlmostYUL.R =>
     phoare[ AlmostYul._REDC :
-                 0 <=(comb Tlo Thi) < R_in * N /\ arg = (Tlo, Thi, R_in, N, N') ==> res = (comb Tlo Thi) * inv N R_in %% N] = 1%r.
-admitted.
+                 0 <=(comb Tlo Thi) < R * N /\ arg = (Tlo, Thi, AlmostYUL.R, N, N') /\ 0 <= Thi < R /\
+    0 <= Tlo < R ==> res = (comb Tlo Thi) * inv N AlmostYUL.R %% N] = 1%r.
+progress.
+conseq (almost_yul_redc_full_correctness  (comb Tlo Thi) Tlo Thi AlmostYUL.R N' N _ _ _ _  );auto.
+progress. rewrite /comb. smt. smt. smt.
+qed.    
 
 
 lemma qq (x a b : int) : 0 < b < a => 0  <= x =>
@@ -51,32 +83,30 @@ seq 1 : (#pre /\ hi = a * R2_MOD_P %/ R ). auto. auto.
 seq 1 : (#pre /\ lo = a * R2_MOD_P %% R). auto. auto.
 exists* lo, hi. elim*. move => loL hiL.
 simplify.
-call  (almost_yul_redc_full_correctness' loL hiL  R N' P). smt. smt. smt. smt.
+call  (almost_yul_redc_full_correctness' loL hiL  N' P). smt. smt. smt. smt.
 skip. progress.
 rewrite /comb. smt.
 apply comb_lemma.
 split. smt. smt.
-split. smt.
-progress.
-have q1 : a{hr} * R2_MOD_P %/ R <= a{hr} * R2_MOD_P %/ (2 * P). apply qq. smt.
-smt.
-have q2 : a{hr} * R2_MOD_P %/ (2 * P) <= a{hr}  %/ 2 . smt.
-have q3 : a{hr}  %/ 2 <= P - 1 .  smt.
-smt.
+split. smt. smt. smt. smt. smt. smt. 
 rewrite /comb.
 have ->: (a{hr} * R2_MOD_P %/ R * R + a{hr} * R2_MOD_P %% R)
  = (a{hr} * R2_MOD_P). smt.
 rewrite ax6.
 have ->: a{hr} * (R * R %% Top.P) * inv Top.P R
  = a{hr} * ((R * R %% Top.P) * inv Top.P R). smt.
-
 have ->: a{hr} * (R * R %% Top.P * inv Top.P R) %% Top.P
  = a{hr} %% Top.P * (R * R %% Top.P * inv Top.P R %% Top.P) %% Top.P. smt(@Int @IntDiv).
-admit.
-
+have ->: (R * R %% P * inv P R %% P) = (R * R * inv P R %% P). smt(@Int @IntDiv).
+have ->: (R * R * inv P R %% P) = (R * (R * inv P R) %% P). smt(@Int @IntDiv).
+have ->: (R * (R * inv P R) %% P) = (R * ((inv P R * R ) %% P) %% P). smt(@Int @IntDiv). rewrite inv_ax. smt.
+ smt(@Int @IntDiv).
 hoare. simplify. auto. auto.
 hoare. simplify. auto. auto.
 qed. 
+
+
+
 
 
 lemma outof_m m_in :
@@ -84,8 +114,8 @@ lemma outof_m m_in :
 proc.
 exists* m. elim*. move => mL.
 simplify.
-call  (almost_yul_redc_full_correctness' mL 0  R N' P). smt. smt. smt. smt.
-skip. progress. smt. smt.
+call  (almost_yul_redc_full_correctness' mL 0   N' P);auto. smt. smt. smt. smt.
+progress. smt. smt. smt. smt.
 qed.    
 
 
@@ -131,16 +161,16 @@ seq 2 : (#pre /\ higherHalfOfProduct = ((a_in * R %% P) * (b_in * R %% P)) %/ R 
 auto. wp. skip. progress.
 exists* lowestHalfOfProduct, higherHalfOfProduct. elim*.
 move => lo hi.
-call  (almost_yul_redc_full_correctness' lo hi  R N' P). smt. smt. smt. smt.
+call  (almost_yul_redc_full_correctness' lo hi  N' P). smt. smt. smt. smt.
 skip. progress. 
 smt.
 have ->: comb (a_in * R %% P * (b_in * R %% P) %% R)
   (a_in * R %% P * (b_in * R %% P) %/ R)
    = a_in * R %% P * (b_in * R %% P). smt.
-smt.
+smt. smt. smt. smt. smt.
 have ->: comb (a_in * R %% P * (b_in * R %% P) %% R)
   (a_in * R %% P * (b_in * R %% P) %/ R)
-   = a_in * R %% P * (b_in * R %% P). smt.
+   = a_in * R %% P * (b_in * R %% P). timeout 10. smt.
 have ->:
    a_in * R %% P * (b_in * R %% P) * inv P R %% P
  =  a_in * R  * ((b_in * R %% P) * inv P R) %% P.
@@ -166,3 +196,166 @@ have ->: a_in * R * (b_in %% P) %% P
 smt().
 hoare. simplify. wp. skip. progress. auto.
 qed.  
+
+
+require import Ext_gcd_optmized.
+
+lemma inv_eq u_in :
+     equiv [ AlmostYul.simplify_ts_pos ~ OptExtGcd.simplify_ts_pos : ={t2,t3,u} /\ u{1} = u_in
+       /\ 0 <= t2{1} <= u{1}  /\ 0 <= t3{1} <= u{1} /\ 2 * u{1} < R /\ 0 <= u{1} ==> ={res} /\ 0 <= res{1}.`1 <= u_in /\ 0 <= res{1}.`2 <= u_in ].
+proc. simplify.
+while (#pre). wp. skip. progress.
+smt. smt. smt. smt. smt. smt. smt. smt. smt.
+skip. progress.
+qed.    
+    
+
+lemma simp_eq :
+     equiv [ AlmostYul.binaryExtendedEuclideanAlgorithm ~ OptExtGcd.main10 : ={arg} /\ 0 < u{1} /\ 0 <= r{1} <= u{2} /\ 0 < v{2} < u{2} /\ 2 * u{1} < R ==> res{1} = res{2}.`1   ].
+proc. simplify.
+while (={u2,v2,t2,u3,v3,t3,u,v,r} 
+  /\ 0 <= u2{1} <= u{1}
+  /\ 0 <= v2{1} <= u{1}
+  /\ 0 <= t2{1} <= u{1}
+  /\ 0 <= u3{1} <= u{1}
+  /\ 0 <= v3{1} <= u{1}
+  /\ 0 <= t3{1} <= u{1}       
+  /\ 2 * u{1}   < R
+  /\ 0 < v{1} < u{1}
+  /\ 0 < u{1} 
+).
+seq 1 1 : (={u2,v2,t2,u3,v3,t3,u,v,r} 
+  /\ 0 <= u2{1} <= u{1}
+  /\ 0 <= v2{1} <= u{1}
+  /\ 0 <= t2{1} <= u{1}
+  /\ 0 <= u3{1} <= u{1}
+  /\ 0 <= v3{1} <= u{1}
+  /\ 0 <= t3{1} <= u{1}       
+  /\ 2 * u{1}   < R
+  /\ 0 < v{1} < u{1}
+  /\ 0 < u{1} ).
+ecall (inv_eq  u{1}). simplify. skip. progress.
+smt.
+wp. skip. progress;smt.
+seq 3 3 : (={u2,v2,t2,u3,v3,t3,u,v,r} 
+  /\ 0 <= u2{1} <= u{1}
+  /\ 0 <= v2{1} <= u{1}
+  /\ 0 <= t2{1} <= u{1}
+  /\ 0 <= u3{1} <= u{1}
+  /\ 0 <= v3{1} <= u{1}
+  /\ 0 <= t3{1} <= u{1}       
+  /\ 2 * u{1}   < R
+  /\ 0 < v{1} < u{1}
+  /\ 0 < u{1} ).
+wp. skip. progress;smt().
+seq 1 1 : (={u2,v2,t2,u3,v3,t3,u,v,r} 
+  /\ 0 <= u2{1} <= u{1}
+  /\ 0 <= v2{1} <= u{1}
+  /\ 0 <= t2{1} <= u{1}
+  /\ 0 <= u3{1} <= u{1}
+  /\ 0 <= v3{1} <= u{1}
+  /\ 0 <= t3{1} <= u{1}       
+  /\ 2 * u{1}   < R
+  /\ 0 < v{1} < u{1}
+  /\ 0 < u{1} ).
+ecall (inv_eq  u{1}). simplify. wp. skip. progress;smt.
+wp. skip. progress;smt.
+qed.
+
+
+
+
+
+lemma inv_m a_in :
+       phoare [ AlmostYul.montgomeryModularInverse : arg = (a_in * R %% P)  /\ 0 < arg < P
+         ==> res = (inv P a_in) * R %% P ] = 1%r.
+bypr. progress. rewrite H. rewrite H in H0. rewrite H in H1. clear H.
+ have ->: Pr[AlmostYul.montgomeryModularInverse(a_in * R %% P) @ &m : res = inv P a_in * R %% P]
+        = Pr[AlmostYul.binaryExtendedEuclideanAlgorithm(P, a_in * R %% P, R2_MOD_P) @ &m : res = inv P a_in * R %% P].
+  byequiv. proc*. inline AlmostYul.montgomeryModularInverse. wp. sp. simplify.
+   call (_:true). sim. skip. progress. auto. auto.
+        
+ have ->: Pr[AlmostYul.binaryExtendedEuclideanAlgorithm(P, a_in * R %% P, R2_MOD_P) @ &m : res = inv P a_in * R %% P]
+        = Pr[OptExtGcd.main10(P, a_in * R %% P, R2_MOD_P) @ &m :
+   res.`1 = inv P a_in * R %% P].
+byequiv. conseq  simp_eq. progress. smt. smt. smt. smt. auto. auto. auto.
+
+byphoare (_: arg = (P, a_in * R %% P, R2_MOD_P) ==> _).
+conseq (modular_inversion_correctness P (a_in * R %% P) R2_MOD_P _ _ _ _ _ _).
+have QQ : inv P a_in * R %% P = inv P (a_in * R %% P) * R2_MOD_P %% P.
+
+  have ->: inv P (a_in * R %% P) * R2_MOD_P %% P = inv P (a_in * R %% P) %% P * R2_MOD_P %% P.
+  smt(@Int @IntDiv). rewrite ax12. rewrite ax13. apply prime_coprime. smt. smt.
+          rewrite ax11.  rewrite ax13. apply prime_coprime. smt. smt.
+have ->: inv P a_in * inv P R %% P = (inv P a_in %% P) * (inv P R %% P) %% P.   smt(@Int @IntDiv).
+have ->: inv P a_in %% P * (inv P R %% P) %% P * R2_MOD_P %% P
+        = inv P a_in %% P * (inv P R %% P) * R2_MOD_P %% P. smt(@Int @IntDiv).
+
+
+rewrite  ax6.
+have ->: inv P a_in %% P * (inv P R %% P) * (R * R %% P) %% P
+     = inv P a_in %% P * ((inv P R %% P) * (R * R %% P)) %% P. smt().
+have ->: inv P a_in %% P * ((inv P R %% P) * (R * R %% P)) %% P
+   = inv P a_in %% P * ((inv P R %% P) * (R * R %% P) %% P) %% P. smt(@Int @IntDiv).
+have ->:  R * R %% P  =  R %% P * R %% P. smt(@Int @IntDiv).
+have ->: (inv P R %% P * (R %% P * R %% P) %% P) =
+   (inv P R %% P * (R %% P * R) %% P). smt(@Int @IntDiv).
+have ->: inv P R %% P * (R %% P * R) = (inv P R %% P * (R %% P)) * R.   smt().
+have ->: (inv P R %% P * (R %% P) * R %% P) = (inv P R %% P * (R %% P) %% P * R %% P).   smt(@Int @IntDiv).
+have ->: inv P R %% P * (R %% P) %% P = inv P R  * R %% P. smt(@Int @IntDiv).
+rewrite inv_ax. smt.  simplify.   
+smt(@Int @IntDiv). 
+progress.
+rewrite H. apply QQ. rewrite H. rewrite  QQ. auto.
+rewrite /P.   smt. smt. smt.  smt.
+apply prime_coprime. smt. smt. smt. auto. auto. qed.
+
+lemma div_m a_in b_in :
+       phoare [ AlmostYul.montgomeryDiv : arg = (a_in * R %% P, b_in * R %% P)  /\ 0 <= arg.`1 < P
+           /\  0 < arg.`2 < P
+         ==> res =  a_in * (inv P b_in) * R %% P ] = 1%r.
+proc. simplify.
+seq 1 : (#pre /\ inverse = (inv P b_in) * R %% P ) 1%r 1%r 0%r 0%r.  auto.
+exists* divisor. elim*. move => div_v.
+call (inv_m b_in).               skip. progress.
+call (mul_m a_in (inv P b_in)). skip. progress.
+smt. smt. 
+phoare split ! 1%r 1%r.
+auto.        
+call (inv_m b_in).               skip. progress.
+call (inv_m b_in).               skip. progress.           
+auto.
+qed.       
+
+
+
+lemma into_m_h m_in :
+ hoare [ AlmostYul.intoMontgomeryForm : arg = m_in  /\ 0 <= a < P ==> res = (m_in * R) %% P ].
+hoare.
+phoare split ! 1%r 1%r. auto. proc. inline*. auto.
+apply into_m. qed.
+
+
+lemma mul_m_h a_in b_in :
+       hoare [ AlmostYul.montgomeryMul : arg = (a_in * R %% P,b_in * R %% P)  /\ 0 <= arg.`1 < P
+         /\  0 <= arg.`2 < P ==> res = (a_in * b_in) * R %% P ].
+hoare.
+phoare split ! 1%r 1%r. auto. proc. inline*. auto.
+apply mul_m. qed.
+
+lemma div_m_h a_in b_in :
+       hoare [ AlmostYul.montgomeryDiv : arg = (a_in * R %% P, b_in * R %% P)  /\ 0 <= arg.`1 < P
+           /\  0 < arg.`2 < P
+         ==> res =  a_in * (inv P b_in) * R %% P ].
+hoare.
+phoare split ! 1%r 1%r. auto. proc*.  call (div_m a_in b_in). progress.
+apply div_m. qed.
+
+lemma submod_h a_in b_in m_in :
+    hoare [ AlmostYul.submod : arg = (a_in,b_in,m_in)  /\ 0 <= a_in < m_in /\ 0 <= 2 * m_in < R
+      /\  0 <= b_in <= m_in ==> res = (a_in - b_in) %% m_in ]. admitted.
+
+
+lemma outof_m_h m_in :
+    hoare [ AlmostYul.outOfMontgomeryForm : arg = m_in  /\ 0 <= m < P ==> res = m_in * (inv P R) %% P ].
+admitted.
