examples/ecAdd/proofs/opt_redc.ec
@@ -214,14 +214,11 @@ qed.
 lemma almost_yul_redc_full_correctness T_in Tlo Thi R_in N' N :
   2 * N < R_in =>
   0 < N => 
-  0 <= T_in < R_in * N =>
   (N' * N %% R_in) = (- 1) %% R_in => 
   coprime N R_in =>
-  Tlo = T_in %% R_in =>
-  Thi = T_in %/ R_in =>
   
  phoare[ AlmostYul._REDC : 
-         arg = (Tlo,Thi,R_in,N,N')
+         arg = (Tlo,Thi,R_in,N,N') /\  Tlo = T_in %% R_in /\ Thi = T_in %/ R_in /\ 0 <= T_in < R_in * N
               ==> res = T_in * (inv N R_in) %% N ] = 1%r.
       
 proof. progress. bypr. progress.
